\section{Ableitungen}

Regeln:\\
\begin{itemize}
    \item Produktregel: $f'*g+f*g'$
    \item Kettenregel: algemein: $\textcolor{red}{g(}f(x\textcolor{red}{)} = \textcolor{red}{g'(}f(x)\textcolor{red}{)}*f'(x)$\\
          $y=\textcolor{red}{(}x^2\textcolor{red}{)^3} \rightarrow y'=\textcolor{red}{3*(}x^2\textcolor{red}{)^2} \rightarrow y'=6x*(x^2)^2 = 6x^5$
    \item Potenzregel: $y=\sqrt{x} = x^\frac{1}{2} \rightarrow \frac{1}{2}*x^{-\frac{1}{2}} = \frac{1}{2}*\frac{1}{x^\frac{1}{2}} = \frac{1}{2\sqrt{x}}$
\end{itemize}


\hfill \break
\input{Topics/Ableitungen/SubTopics/GraphischesAbleiten}
\break
\input{Topics/Ableitungen/SubTopics/GraphischesAbleitenBeispiele}
\break
\input{Topics/Ableitungen/SubTopics/FunktionAufstellen}
\break
\input{Topics/Ableitungen/SubTopics/Kurvendiskussion}
\break
\input{Topics/Ableitungen/SubTopics/Uebersetzungshilfe}
\break
\input{Topics/Ableitungen/SubTopics/AbleitungEinigerAnderenFunktionen}